src/lib/kuiper/Kuiper.Kernel.Base.fsti
@@ -20,9 +20,92 @@ val shmem_tok
   (ar:gpu_array a sz)
 : slprop
 
+noeq
+inline_for_extraction noextract
+type kernel_desc = {
+  nblk : (x : SZ.t { 0 < x /\ x <= max_blocks });
+  nthr : (x : SZ.t { 0 < x /\ x <= max_threads });
+
+  shmem_type : Type u#0;
+  shmem_type_is_sized : Kuiper.Sized.sized shmem_type;
+  shmem_sz : sz;
+
+  (* This is used to split up the array for the threads in the block.
+     It should definitely be generalized to be more uniform with
+     other levels of the hierarchy, e.g. by having a teardown. Currently
+     we just drop the block_post. *)
+  block_pre  : gpu_array shmem_type shmem_sz -> natlt nblk -> natlt nthr -> slprop;
+  block_post : gpu_array shmem_type shmem_sz -> natlt nblk -> natlt nthr -> slprop;
+  block_setup : (
+    (ar: gpu_array shmem_type shmem_sz) ->
+    (bid: natlt nblk) ->
+    stt_ghost unit emp_inames
+      (requires
+        block_setup nthr **
+        (exists* v. gpu_pts_to_array #shmem_type #shmem_sz ar #1.0R v))
+      (ensures fun _ ->
+        block_setup nthr **
+        (forall+ (i : natlt nthr). block_pre ar bid i))
+  );
+
+  kpre : natlt nblk -> natlt nthr -> slprop;
+  kpost : natlt nblk -> natlt nthr -> slprop;
+
+  f : (
+    eshmem : erased (gpu_array shmem_type shmem_sz) ->
+    ebid : enatlt nblk ->
+    etid : enatlt nthr ->
+    stt unit
+      (requires
+         gpu **
+         kpre ebid etid **
+         thread_id nthr etid **
+         block_id nblk ebid **
+         shmem_tok eshmem **
+         block_pre eshmem ebid etid
+      )
+      (ensures fun _ ->
+         gpu **
+         kpost ebid etid **
+         thread_id nthr etid **
+         block_id nblk ebid **
+         shmem_tok eshmem **
+         block_post eshmem ebid etid)
+  );
+  full_pre : slprop;
+  setup : (
+    unit ->
+    stt_ghost unit emp_inames
+      (requires full_pre)
+      (ensures  fun _ -> forall+ (bid : natlt nblk) (tid : natlt nthr). kpre bid tid)
+  );
+  full_post : slprop;
+  teardown : (
+    unit ->
+    stt_ghost unit emp_inames
+      (requires forall+ (bid : natlt nblk) (tid : natlt nthr). kpost bid tid)
+      (ensures  fun _ -> full_post)
+  );
+}
+
 (* This is the single primitive for launching kernels, with the most general
 type and capabilities. There are many simpler versions in the Kuiper.Kernel module,
 all implemented using this one and without any extra assumptions. *)
+fn launch_kernel (k : kernel_desc)
+  (#e : epoch_t)
+  requires
+    cpu **
+    epoch_live e **
+    k.full_pre
+  returns
+    e' : epoch_t
+  ensures
+    cpu **
+    epoch_live e' **
+    pledge0 (epoch_done e') k.full_post **
+    pure (e' >= e)
+
+inline_for_extraction noextract
 fn launch_kernel_n_m_shmem_async
   (nblk : szp { nblk <= max_blocks })
   (nthr : szp { nthr <= max_threads })
